Mostly finish HashMap impl

LeanColls/FoldableOps.lean
@@ -5,23 +5,53 @@ Authors: James Gallicchio
 -/
 
 import LeanColls.Classes
+import LeanColls.FoldableCorrect
+import LeanColls.List.Basic
 
 namespace LeanColls
 
-class FoldableOps (C τ) [Foldable C τ] where
+class FoldableOps.{uC,uT} (C : Type uC) (τ : Type uT) where
   toList : C → List τ
   all : C → (τ → Bool) → Bool
   contains : C → [BEq τ] → τ → Bool
-  sum : C → [Add τ] → [OfNat τ 0] → τ
+  sum : C → [AddMonoid τ] → τ
 
 namespace FoldableOps
 
-def defaultImpl (F : Foldable C τ) : FoldableOps C τ where
-  toList    := λ c      => Foldable.fold c (fun acc x => x::acc) [] |>.reverse
-  all       := λ c f    => Foldable.fold c (fun acc x => acc && f x) true
-  contains  := λ c _ x  => Foldable.fold c (fun acc y => acc || BEq.beq x y) true
-  sum       := λ c      => Foldable.fold c (fun acc x => acc + x) 0
+def defaultImpl (C : Type u) (τ : Type v) [Foldable C τ] : FoldableOps C τ where
+  toList := λ c =>
+    Foldable.fold c (fun acc x => x::acc) []
+    |>.reverse
+  all := λ c f =>
+    Foldable.fold c (β := ULift Bool) (fun acc x => ⟨acc.down && f x⟩) ⟨true⟩
+    |>.down
+  contains := λ c _ x  =>
+    Foldable.fold c (β := ULift Bool) (fun acc y => ⟨acc.down || BEq.beq x y⟩) ⟨true⟩
+    |>.down
+  sum := λ c =>
+    Foldable.fold c (fun acc x => acc + x) 0
 
-instance [F : Foldable C τ] : Inhabited (FoldableOps C τ) where
-  default := defaultImpl F
+instance [Foldable C τ] : Inhabited (FoldableOps C τ) where
+  default := defaultImpl C τ
 
+theorem sum_eq_sum_toList [F : Foldable.Correct C τ] [FoldableOps C τ] [AddMonoid τ] (c : C)
+  (h : FoldableOps.sum c = (defaultImpl C τ).sum c := by rfl)
+  : FoldableOps.sum c = List.sum (canonicalToList (Foldable.fold c))
+  := by
+  simp [autoParam] at h
+  rw [h]
+  simp [defaultImpl, sum]
+  rw [Foldable.Correct.foldCorrect]
+  generalize canonicalToList _ = list
+  simp [List.fold]
+  suffices ∀ (acc : τ) list, List.foldl (fun acc x => acc + x) acc list = acc + List.sum list by
+    have := this 0 list
+    simp at this
+    exact this
+  intro acc list
+  induction list generalizing acc with
+  | nil =>
+    simp [List.foldl, List.sum]
+  | cons x xs ih =>
+    simp [List.foldl, List.sum, ih]
+    rw [AddMonoid.toAddSemigroup.add_assoc]
