LeanColls/View.lean
@@ -10,33 +10,40 @@ import LeanColls.FoldableCorrect
 
 namespace LeanColls
 
-structure View (τ) where
-  fold : {β : Type w} → (β → τ → β) → β → β
+/-! # View
+
+Isomorphic to a `(Foldable C τ) × C`; a fold instantiated
+at a specific collection. Used to implement inline transformations
+which are only evaluated when the collection is folded into a result.
+-/
+structure View.{u,v} (τ : Type u) where
+  fold : {β : Type v} → (β → τ → β) → β → β
 
 namespace View
 
-instance : Foldable (View τ) τ where
-  fold c f acc := c.fold f acc
+@[inline]
+instance : Foldable.{max u (v+1),u,v} (View.{u,v} τ) τ where
+  fold v f acc := v.fold f acc  
 
-instance [BEq τ] : FoldableOps (View τ) τ := default
+@[inline]
+instance : FoldableOps (View τ) τ := FoldableOps.defaultImpl (View τ) τ  
 
-@[inline,reducible]
+@[inline]
 def view {F τ} (c : F) [Foldable F τ] : View τ where
-  fold f acc := Foldable.fold c f acc
+  fold := λ f acc => Foldable.fold c f acc
 
-@[inline,reducible]
+@[inline]
 def map {τ : Type u} {τ' : Type v} (f : τ → τ') (v : View τ) : View τ' where
-  fold foldF foldAcc :=
-    v.fold (λ acc t => foldF acc (f t)) foldAcc
+  fold := λ foldF foldAcc => v.fold (λ acc t => foldF acc (f t)) foldAcc
 
-@[inline,reducible]
+@[inline]
 def filter (f : τ → Bool) (v : View τ) : View τ where
-  fold foldF foldAcc :=
+  fold := λ foldF foldAcc =>
     v.fold (λ a x =>
       if f x then foldF a x else a
     ) foldAcc
 
-@[inline,reducible]
+@[inline]
 def filterMap (f : τ → Option τ') (v : View τ) : View τ' where
   fold := λ foldF foldAcc =>
     v.fold (λ a x =>
@@ -44,8 +51,6 @@ def filterMap (f : τ → Option τ') (v : View τ) : View τ' where
       | none    => a
       | some x' => foldF a x'
     ) foldAcc
-
-instance : FoldableOps (View τ) τ := default
 
 structure WithMem (τ) (c : C) (M : outParam (Membership τ C)) where
   fold' : {β : Type w} → (β → (x : τ) → x ∈ c → β) → β → β
@@ -63,13 +68,12 @@ def map' {τ : Type u} {c : C} {M} (v : View.WithMem τ c M) {τ' : Type v} (f :
 
 end WithMem
 
-
 theorem canonicalToList_map [Foldable.Correct C τ] (c : C) (f : τ → τ')
   : canonicalToList (((View.view c).map f).fold)
     = List.map f (canonicalToList (Foldable.fold c))
   := by
   generalize h : canonicalToList (Foldable.fold c) = list
-  simp [canonicalToList]
+  simp [canonicalToList, view, map]
   rw [Foldable.Correct.foldCorrect, h]
   clear h c
   simp [List.fold]
@@ -90,20 +94,21 @@ theorem canonicalToList_filter [Foldable.Correct C τ] (c : C) (f)
     = List.filter f (canonicalToList (Foldable.fold c))
   := by
   generalize h : canonicalToList (Foldable.fold c) = list
-  simp [canonicalToList]
+  simp [canonicalToList, view, filter]
   rw [Foldable.Correct.foldCorrect, h]
   clear h c
   simp [List.fold]
+  rw [List.filter_eq_filterTR]
   suffices ∀ init,
     List.foldl (fun acc t => if f t = true then acc ++ [t] else acc) init list
-      = List.filterAux f list init.reverse
+      = List.filterTRAux f list init.reverse
     from this []
   intro init
   induction list generalizing init with
   | nil =>
-    simp [List.foldl, List.filter, List.filterAux]
+    simp [List.foldl, List.filter, List.filterTRAux]
   | cons x xs ih =>
-    simp [List.foldl, List.filter, List.filterAux]
+    simp [List.foldl, List.filter, List.filterTRAux]
     split
     case inl h =>
       simp [h]
